Experiments/SR/Checker/SRThm.lean
@@ -1,0 +1,893 @@
+/-
+Copyright (c) 2024 The Trestle Contributors.
+Released under the Apache License v2.0; see LICENSE for full text.
+-/
+
+import Experiments.SR.Checker.SRChecker
+import Experiments.SR.Data.PPA.Thm
+import Experiments.SR.Data.PS.Thm
+import Experiments.SR.Data.RangeArray.Thm
+import Trestle.Model.PropFun
+import Trestle.Data.Cnf.Basic
+import Trestle.Data.ICnf.Basic
+
+namespace Trestle.SR
+
+open RangeArray PPA PS
+open Trestle Trestle.Model PropFun
+open Except
+
+/-
+
+  We model `RangeArray`s with a list of `Option (List ILit)` for the formula
+  clauses and a `List ILit` for the candidate redudant clause.
+
+  We need a way of converting those into `PropFun`. We manually define
+  that transformation here.
+
+  Note that we assume "empty"/deleted clauses are `⊤` instead of `⊥`.
+
+-/
+
+private def clauseAsListToPropFun (C : List ILit) : PropFun IVar :=
+  Clause.toPropFun { toList := C }
+
+private def cnfAsListToPropFun (Cs : List (Option (List ILit))) : PropFun IVar :=
+  .all (Cs.map (fun C =>
+    match C with
+    | none => ⊤
+    | some C => clauseAsListToPropFun C))
+
+@[simp]
+theorem clauseAsListToPropFun_eq_toPropFun (C : List ILit)
+    : clauseAsListToPropFun C = Clause.toPropFun ({ toList := C } : IClause) :=
+  rfl
+
+-- To avoid the empty clause problem, we use `[1, ¬1]`.
+theorem cnfAsListToPropFun_eq_toPropFun (Cs : List (Option (List ILit)))
+    : cnfAsListToPropFun Cs = Cnf.toPropFun ({ toList := Cs.map (fun cl =>
+        match cl with
+        | none => { toList := [LitVar.mkPos 1, LitVar.mkNeg 1] }
+        | some C => { toList := C }) } : ICnf) := by
+  simp [cnfAsListToPropFun]
+  induction Cs with
+  | nil => simp
+  | cons C Cs ih =>
+    match C with
+    | none => simp [ih]
+    | some C => simp [← ih, PropFun.all]
+
+@[simp]
+theorem cnfAsListToPropFun_nil : cnfAsListToPropFun [] = ⊤ := by
+  simp [cnfAsListToPropFun]
+
+@[simp]
+theorem cnfAsListToPropFun_cons_none (Cs : List (Option (List ILit))) :
+  cnfAsListToPropFun (none :: Cs) = cnfAsListToPropFun Cs := by
+  simp [cnfAsListToPropFun, all]
+
+@[simp]
+theorem cnfAsListToPropFun_cons_some (C : List ILit) (Cs : List (Option (List ILit))) :
+  cnfAsListToPropFun (some C :: Cs) = clauseAsListToPropFun C ⊓ cnfAsListToPropFun Cs := by
+  simp [cnfAsListToPropFun, all]
+
+@[simp]
+theorem cnfAsListToPropFun_cons (C : Option (List ILit)) (Cs : List (Option (List ILit))) :
+  cnfAsListToPropFun (C :: Cs) =
+    (match C with
+    | none => ⊤
+    | some C => clauseAsListToPropFun C) ⊓ cnfAsListToPropFun Cs := by
+  cases C <;> simp
+
+@[simp]
+theorem cnfAsListToPropFun_append (Cs₁ Cs₂ : List (Option (List ILit))) :
+  cnfAsListToPropFun (Cs₁ ++ Cs₂) = cnfAsListToPropFun Cs₁ ⊓ cnfAsListToPropFun Cs₂ := by
+  induction Cs₁ with
+  | nil => simp
+  | cons C Cs₁ ih =>
+    simp [List.append]
+    cases C <;> simp [ih, inf_assoc]
+
+@[simp]
+theorem cnfAsListToPropFun_replicate_none (n : Nat) :
+    cnfAsListToPropFun (List.replicate n none) = ⊤ := by
+  induction n with
+  | zero => simp
+  | succ n ih =>
+    simp [List.replicate]
+    exact ih
+
+theorem clausePropFun_ge_of_mem {C : List ILit} {l : ILit}
+    : l ∈ C → l.toPropFun ≤ clauseAsListToPropFun C := by
+  intro h
+  rw [clauseAsListToPropFun_eq_toPropFun]
+  apply Clause.toPropFun_mem_le
+  simp only [Array.mem_toArray, h]
+
+theorem cnfPropFun_le_of_mem {Cs : List (Option (List ILit))} {C : List ILit} {i : Nat}
+      {hi : i < Cs.length} :
+    Cs.get ⟨i, hi⟩ = some C → cnfAsListToPropFun Cs ≤ clauseAsListToPropFun C := by
+  intro h
+  simp [cnfAsListToPropFun_eq_toPropFun]
+  induction Cs generalizing i with
+  | nil => simp at hi
+  | cons X Xs ih =>
+    match X with
+    | none =>
+      match i with
+      | 0 => simp at h
+      | i + 1 =>
+        simp at hi h
+        simp [ih h]
+    | some X =>
+      match i with
+      | 0 =>
+        simp at h; subst h
+        simp [clauseAsListToPropFun_eq_toPropFun]
+      | i + 1 =>
+        simp at h
+        have := ih h
+        apply le_trans _ this
+        simp
+
+theorem cnfPropFun_le_set_none {Cs : List (Option (List ILit))}
+  {i : Nat} (hi : i < Cs.length) :
+    cnfAsListToPropFun Cs ≤ cnfAsListToPropFun (Cs.set i none) := by
+  induction Cs generalizing i with
+  | nil => contradiction
+  | cons C Cs ih =>
+    cases i with
+    | zero => simp [List.set]
+    | succ i =>
+      simp [List.set]
+      simp at hi
+      apply le_trans _ (ih hi)
+      cases C <;> simp
+
+theorem list_satisfies_iff {τ : PropAssignment IVar} {Cs : List (Option (List ILit))} :
+    τ ⊨ cnfAsListToPropFun Cs ↔ ∀ {C : List ILit}, (some C) ∈ Cs → τ ⊨ clauseAsListToPropFun C := by
+  simp [cnfAsListToPropFun_eq_toPropFun]
+  induction Cs with
+  | nil => simp
+  | cons C Cs ih =>
+    match C with
+    | none => simp [ih]
+    | some C =>
+      simp at ih ⊢
+      intro _
+      exact ih
+
+/-! # Correctness -/
+
+theorem assumeNegatedCandidateFor.loop.aux {F : RangeArray ILit} {τ : PPA} {Ls : List (Option (List ILit))} {L : List ILit}
+    (h_models : models F Ls L) {bumps : Nat} {i j : Nat}
+  : j = L.length - i →
+    assumeNegatedCandidateFor.loop F bumps (F.dsize + i) τ = assumeNegatedClauseFor.loop { toList := L } bumps i τ := by
+  intro hj
+  induction j generalizing τ i with
+  | zero =>
+    have h_le₁ := Nat.le_of_sub_eq_zero hj.symm
+    have h_le₂ := h_models.h_size₂.symm ▸ h_le₁
+    unfold assumeNegatedClauseFor.loop
+    simp at h_le₂ ⊢
+    simp [not_lt.mpr h_le₁]
+    unfold assumeNegatedCandidateFor.loop
+    simp [not_lt.mpr h_le₂]
+    intro h
+    omega
+  | succ j ih =>
+    unfold assumeNegatedClauseFor.loop
+    have hi : i < List.length L := by
+      apply Nat.lt_of_sub_pos
+      rw [← hj]
+      exact Nat.zero_lt_succ j
+    simp [hi]
+    have h_agree := h_models.h_uncommitted hi
+    simp [uget] at h_agree
+    have := h_models.h_size₂
+    rw [← this, usize] at hi
+    split <;> rename _ => h_get
+    · rw [← @ih (setLitFor τ (-L[i]) bumps) (i + 1) (by omega)]
+      rw [assumeNegatedCandidateFor.loop]
+      have : F.dsize + i < F.data.size := by omega
+      simp [this, hi, h_get, h_agree, Nat.add_assoc]
+    · rw [← @ih τ _ (by omega)]
+      rw [assumeNegatedCandidateFor.loop]
+      split <;> rename _ => hi'
+      · simp [h_agree, h_get, Nat.add_assoc]
+      · have := h_models.h_size₂
+        rw [usize] at this
+        omega
+    · rw [assumeNegatedCandidateFor.loop]
+      split <;> rename _ => hi'
+      · simp [h_agree, h_get]
+      · omega
+
+@[simp]
+theorem assumeNegatedCandidateFor_eq_assumeNegatedClauseFor {F : RangeArray ILit}
+      {Ls : List (Option (List ILit))} {L : List ILit} (τ : PPA) (bumps : Nat)
+  : models F Ls L →
+    assumeNegatedCandidateFor F τ bumps = assumeNegatedClauseFor τ ({ toList := L} : IClause) bumps := by
+  intro h_models
+  simp [assumeNegatedCandidateFor, assumeNegatedClauseFor]
+  exact @assumeNegatedCandidateFor.loop.aux _ _ _ _ h_models bumps 0 F.usize h_models.h_size₂
+
+theorem assumeRATClause.loop.aux {F : RangeArray ILit} {τ : PPA} {σ : PS}
+    {Ls : List (Option (List ILit))} {L : List ILit} (h_models : models F Ls L)     -- models
+    {i : Nat} (hi : i < F.size)                                                     -- Clause index
+    {C : List ILit} (hC : Ls.get ⟨i, h_models.h_size₁ ▸ hi⟩ = some C)               -- Clause at i
+    {j k : Nat}
+  : k = C.length - j →
+    match assumeRATClause.loop F i σ ((F.index i hi) + j) τ with
+    -- If we exit early, then τ satisfies the clause under the substitution, and τ is unchanged
+    | .error τ' => τ.toPropFun ≤ PropFun.substL (clauseAsListToPropFun ((C.drop j))) σ.toSubst ∧ extendsFor τ τ' 0
+    -- If we make it to the end, then τ' has been assumed by the negated candidate under the substitution
+    | .ok τ' => τ'.toPropFun = ↑τ ⊓ (PropFun.substL (clauseAsListToPropFun ((C.drop j))) σ.toSubst)ᶜ ∧ extendsFor τ τ' 0 := by
+  intro hk
+  have hiL := h_models.h_size₁ ▸ hi
+  have hi' := h_models.h_sizes (hiL) hC
+  induction k generalizing τ j with
+  | zero =>
+    have h_le₁ := Nat.le_of_sub_eq_zero hk.symm
+    unfold assumeRATClause.loop
+    have hj := hi' ▸ h_le₁
+    simp [rsize] at hj
+    rw [add_comm j] at hj
+    simp [not_lt_of_ge hj, List.drop_eq_nil_iff.mpr h_le₁]
+  | succ k ih =>
+    unfold assumeRATClause.loop
+    have hj_lt : j < C.length := by omega
+    replace hk : k = C.length - (j + 1) := by omega
+    have : F.index i hi + j < F.index! (i + 1) := by
+      simp [rsize] at hi'
+      omega
+    have hF := h_models.h_agree hiL hC hj_lt
+    rw [oget] at hF
+    simp [this, hF]
+    clear hF
+    match hσ : σ.litValue C[j] with
+    | .inr true =>
+      simp [hσ]
+      have := List.mem_drop_iff_getElem.mpr ⟨0, (by rw [Nat.zero_add]; exact hj_lt), rfl⟩
+      simp [Nat.zero_add] at this
+      have := substL_le_of_le (Clause.toPropFun_mem_list_le this) σ.toSubst
+      apply le_trans _ this
+      simp [PS.litValue_true_iff.mp hσ]
+    | .inr false =>
+      simp [hσ]
+      replace ih := ih (τ := τ) hk
+      split <;> rename_i h_loop
+      <;> simp [h_loop, ← Nat.add_assoc] at ih
+      · rcases ih with ⟨hτ, h_extends⟩
+        constructor
+        · have := Clause.toPropFun_drop_le_drop_of_ge C (Nat.le_succ j)
+          exact le_trans hτ (substL_le_of_le this _)
+        · exact h_extends
+      · rename PPA => τ''
+        rcases ih with ⟨h_eq, h_extends⟩
+        constructor
+        · rw [h_eq, ← List.getElem_cons_drop_succ_eq_drop hj_lt, Clause.toPropFun_cons]
+          simp [litValue_false_iff.mp hσ]
+        · exact h_extends
+    | .inl l' =>
+      simp [PSV.toMappedNat]
+      match hτ : τ.litValue? l' with
+      | none =>
+        simp
+        replace ih := ih (τ := τ.setLitFor (-l') 0) hk
+        have h_neg := litValue?_negate_none_iff.mpr hτ
+        have hτ_le := PPA.toPropFun_setLitFor_le_of_none h_neg 0
+        rw [← List.getElem_cons_drop_succ_eq_drop hj_lt, Clause.toPropFun_cons]
+        simp [← litValue_eq, hσ, PSV.toPropFun]
+        split <;> rename_i h_loop
+        <;> simp [h_loop, ← Nat.add_assoc] at ih
+        <;> rcases ih with ⟨h_eq, h_extends⟩
+        · constructor
+          · simp [toPropFun_setLitFor_of_none h_neg] at h_eq
+            exact inf_compl_le_iff_le_sup.mp h_eq
+          · have := extendsFor_setLitFor_of_none h_neg 0
+            exact extendsFor_trans this h_extends
+        · constructor
+          · simp [h_eq, toPropFun_setLitFor_of_none h_neg, inf_assoc]
+          · have := extendsFor_setLitFor_of_none h_neg 0
+            exact extendsFor_trans this h_extends
+      | some b =>
+        cases b <;> simp
+        -- false branch
+        · replace ih := ih (τ := τ) hk
+          split <;> rename_i h_loop
+          <;> simp [h_loop, ← Nat.add_assoc] at ih
+          <;> simp [ih.2]
+          · have := Clause.toPropFun_drop_le_drop_of_ge C (Nat.le_succ j)
+            exact le_trans ih.1 (substL_le_of_le this _)
+          · simp [ih.1]
+            clear ih
+            rw [← List.getElem_cons_drop_succ_eq_drop hj_lt, Clause.toPropFun_cons]
+            simp [← litValue_eq, hσ, PSV.toPropFun]
+            have := litValue?_false_iff.mp hτ
+            have :  τ.toPropFun ⊓ (LitVar.toPropFun l')ᶜ = τ.toPropFun := by
+              simp [this]
+            rw [← inf_assoc, this]
+        -- true branch
+        · have := Clause.toPropFun_mem_list_le (List.mem_drop_iff_getElem.mpr ⟨0, (by rw [Nat.zero_add]; exact hj_lt), rfl⟩)
+          simp [Nat.add_zero] at this
+          have := litValue?_true_iff.mp hτ
+          rw [← List.getElem_cons_drop_succ_eq_drop hj_lt, Clause.toPropFun_cons]
+          simp [← litValue_eq, hσ, PSV.toPropFun]
+          exact le_sup_of_le_left this
+
+theorem assumeRATClause_result {F : RangeArray ILit} {τ : PPA} {σ : PS}
+    {Ls : List (Option (List ILit))} {L : List ILit} (h_models : models F Ls L)     -- models
+    {i : Nat} (hi : i < F.size)                                                     -- Clause index
+    {C : List ILit} (hC : Ls.get ⟨i, h_models.h_size₁ ▸ hi⟩ = some C)               -- Clause at c_idx
+  : match assumeRATClause F i hi σ τ with
+    | .error τ' => τ.toPropFun ≤ PropFun.substL (clauseAsListToPropFun C) σ.toSubst ∧ extendsFor τ τ' 0
+    | .ok τ' => τ'.toPropFun = ↑τ ⊓ (PropFun.substL (clauseAsListToPropFun C) σ.toSubst)ᶜ ∧ extendsFor τ τ' 0 := by
+  simp [assumeRATClause]
+  exact @assumeRATClause.loop.aux _ _ _ _ _ h_models i hi C hC 0 (C.length) rfl
+
+def unit_to_option (n : Int) : Option ILit :=
+  if hn : n = 0 then none else some ⟨n, hn⟩
+
+@[simp] theorem unit_to_option_zero : unit_to_option 0 = none := by simp [unit_to_option]
+
+theorem unitProp.loop.aux {F : RangeArray ILit} (τ : PPA)
+  {Ls : List (Option (List ILit))} {L : List ILit} (h_models : models F Ls L)     -- models
+  {i : Nat} (hi : i < F.size)                                                     -- Clause index
+  {C : List ILit} (hC : Ls.get ⟨i, h_models.h_size₁ ▸ hi⟩ = some C)               -- Clause at i
+  {j k : Nat} (unit : Int)
+    : k = C.length - j
+        → unitProp.loop τ F i (F.index i hi + j) unit = PPA.unitProp.loop τ { toList := C } j (unit_to_option unit) := by
+  intro hk
+  have hiL := h_models.h_size₁ ▸ hi
+  have hi' := h_models.h_sizes (hiL) hC
+  induction k generalizing τ j unit with
+  | zero =>
+    have hj_le := Nat.le_of_sub_eq_zero hk.symm
+    unfold RangeArray.unitProp.loop
+    unfold PPA.unitProp.loop
+    have hj := hi' ▸ hj_le
+    simp [rsize] at hj
+    rw [add_comm j] at hj
+    simp [not_lt_of_ge hj, not_lt_of_ge hj_le, List.drop_eq_nil_iff.mpr hj_le]
+    split <;> rename _ => h_unit
+    <;> simp [h_unit, unit_to_option]
+  | succ k ih =>
+    have hj_lt : j < C.length := by omega
+    replace hk : k = C.length - (j + 1) := by omega
+    have : F.index i hi + j < F.index! (i + 1) := by
+      simp [rsize] at hi'
+      omega
+    have hF := h_models.h_agree hiL hC hj_lt
+    rw [oget] at hF
+    unfold RangeArray.unitProp.loop
+    unfold PPA.unitProp.loop
+    simp [this, hF, hj_lt]
+    split
+    rename_i lit h_lit hCj
+    simp [hCj]
+    rw [Nat.add_assoc]
+    match hτ : τ.litValue? ⟨lit, h_lit⟩ with
+    | none =>
+      by_cases h_unit : unit = 0
+      <;> simp [h_unit]
+      · simp [unit_to_option, @ih τ (j + 1) lit hk, h_lit]
+      · split <;> rename_i hul
+        · subst hul
+          simp [@ih τ (j + 1) unit hk, unit_to_option, h_lit]
+        · simp [unit_to_option, hul, h_unit]
+          intro h_con
+          injection h_con
+          contradiction
+    | some b =>
+      cases b <;> simp
+      exact @ih τ (j + 1) unit hk
+
+@[simp]
+theorem unitProp_eq_unitProp {F : RangeArray ILit} {τ : PPA}
+  {Ls : List (Option (List ILit))} {L : List ILit} (h_models : models F Ls L)     -- models
+  {i : Nat} (hi : i < F.size)                                                     -- Clause index
+  {C : List ILit} (hC : Ls.get ⟨i, h_models.h_size₁ ▸ hi⟩ = some C)               -- Clause at i
+    : RangeArray.unitProp τ F i hi = PPA.unitProp τ { toList := C } := by
+  simp [RangeArray.unitProp, PPA.unitProp]
+  have := @unitProp.loop.aux _ τ _ _ h_models i hi C hC 0 (C.length) 0 rfl
+  simp at this
+  exact this
+
+theorem applyUPHint_spec {F : RangeArray ILit} {τ : PPA}
+    {Ls : List (Option (List ILit))} {L : List ILit} (h_models : models F Ls L)
+    (hint bumps : Nat)
+  : match applyUPHint F bumps τ hint with
+    | ⟨_, .err⟩ => True
+    | ⟨τ', .unit⟩  =>
+      ∃ (hint : Nat) (h_hint : hint < Ls.length) (C : List ILit), Ls.get ⟨hint, h_hint⟩ = some C
+        ∧ ∃ (lit : ILit), lit ∈ C ∧ τ.litValue? lit = none
+        ∧ τ' = τ.setLitFor lit bumps
+        ∧ (clauseAsListToPropFun C) ⊓ τ = lit.toPropFun ⊓ τ
+        ∧ (cnfAsListToPropFun Ls) ⊓ τ ≤ τ'
+    | ⟨τ', .contra⟩ =>
+      ∃ (hint : Nat) (h_hint : hint < Ls.length) (C : List ILit), Ls.get ⟨hint, h_hint⟩ = some C
+        ∧ τ' = τ
+        ∧ (clauseAsListToPropFun C) ⊓ τ = ⊥ := by
+  simp [applyUPHint]
+  by_cases h_hint : hint < Ls.length
+  · have h_hint' := h_models.h_size₁ ▸ h_hint
+    simp [h_hint']
+    by_cases h_del : F.isDeleted hint h_hint'
+    <;> simp [h_del]
+    simp at h_del
+    rcases (h_models.h_some h_hint).mp h_del with ⟨C, hC⟩
+    rw [unitProp_eq_unitProp h_models h_hint' hC]
+    match h_up : τ.unitProp { toList := C } with
+    | .multipleUnassignedLiterals => simp
+    | .satisfied => simp
+    | .unit ⟨unit, h_unit⟩ =>
+      rw [unitProp_eq_unitPropM] at h_up
+      rcases unitPropM_unit h_up with ⟨h_mem, h_none, hC_inf⟩
+      simp at h_mem
+      simp
+      use hint, h_hint, C, hC, ⟨unit, h_unit⟩, h_mem, h_none
+      simp [hC_inf, toPropFun_setLitFor_of_none h_none bumps]
+      have := cnfPropFun_le_of_mem hC
+      apply le_trans (inf_le_inf_right τ.toPropFun this)
+      simp [Trestle.SR.clauseAsListToPropFun, hC_inf]
+    | .falsified =>
+      simp
+      use hint, h_hint, C, hC
+      rw [unitProp_eq_unitPropM] at h_up
+      exact unitPropM_falsified h_up
+  -- out-of-bounds error branch
+  · have h_hint' := h_models.h_size₁ ▸ h_hint
+    simp [h_hint']
+
+@[simp]
+theorem applyUPHints.nil (F : RangeArray ILit) (τ : PPA) (bumps : Nat)
+  : applyUPHints F bumps τ { toList := [] } = ⟨τ, .unit⟩ := by
+  simp [applyUPHints, applyUPHints.loop]
+
+theorem applyUPHints.loop.cons_succ' (F : RangeArray ILit) (τ : PPA) (bumps hint : Nat)
+    {hints : List Nat} {i j : Nat}
+  : j = hints.length - i →
+    applyUPHints.loop F bumps { toList := hint :: hints } (i + 1) τ = applyUPHints.loop F bumps { toList := hints } i τ := by
+  intro hj
+  induction j generalizing τ i with
+  | zero =>
+    have h_le := Nat.le_of_sub_eq_zero hj.symm
+    unfold applyUPHints.loop
+    simp [not_lt_of_ge h_le]
+  | succ j ih =>
+    have hi : i < hints.length := by
+      apply Nat.lt_of_sub_pos
+      rw [← hj]
+      exact Nat.zero_lt_succ j
+    have hj' : j = hints.length - (i + 1) := by omega
+    unfold applyUPHints.loop
+    simp [hi]
+    match h_hint : applyUPHint F bumps τ hints[i] with
+    | ⟨τ', .err⟩ => simp
+    | ⟨τ', .unit⟩ => simp [ih (τ := τ') hj']
+    | ⟨τ', .contra⟩ => simp [ih (τ := τ') hj']
+
+@[simp]
+theorem applyUPHints.loop.cons_succ (F : RangeArray ILit) (τ : PPA) (bumps hint i : Nat) {hints : List Nat}
+  : applyUPHints.loop F bumps { toList := hint :: hints } (i + 1) τ = applyUPHints.loop F bumps { toList := hints } i τ := by
+  exact @applyUPHints.loop.cons_succ' F τ bumps hint hints i (hints.length - i) (by omega)
+
+theorem applyUPHints_spec {F : RangeArray ILit} {τ : PPA}
+  {Ls : List (Option (List ILit))} {L : List ILit} (h_models : models F Ls L)
+  (bumps : Nat)
+  (hints : List Nat)
+  : match applyUPHints F bumps τ { toList := hints } with
+    | ⟨_, .err⟩ => True
+    | ⟨τ', .unit⟩ => (cnfAsListToPropFun Ls) ⊓ τ ≤ τ' ∧ extendsFor τ τ' bumps
+    | ⟨τ', .contra⟩ => (cnfAsListToPropFun Ls) ⊓ τ = ⊥ ∧ extendsFor τ τ' bumps
+  := by
+  unfold applyUPHints
+  induction hints generalizing τ with
+  | nil => simp [applyUPHints.loop]
+  | cons hint hints ih =>
+    unfold applyUPHints.loop
+    simp
+    match h_hint : applyUPHint F bumps τ hint with
+    | ⟨τ', .err⟩ => simp
+    | ⟨τ', .unit⟩ =>
+      have h_spec := applyUPHint_spec (τ := τ) h_models hint bumps
+      simp [h_hint] at h_spec
+      rcases h_spec with ⟨hint, h_hint_lt, C, hC, lit, h_lit_mem, hτ_lit, hτ', hτ₁, hτ₂⟩
+      simp
+      match h_loop : applyUPHints.loop F bumps { toList := hints } 0 τ' with
+      | ⟨τ'', .err⟩ => simp [h_loop]
+      | ⟨τ'', .unit⟩ =>
+        simp
+        replace ih := ih (τ := τ')
+        subst hτ'
+        simp [h_loop] at ih
+        rcases ih with ⟨ih₁, ih₂⟩
+        constructor
+        · have h : cnfAsListToPropFun Ls ⊓ (cnfAsListToPropFun Ls ⊓ τ.toPropFun)
+                    ≤ cnfAsListToPropFun Ls ⊓ (τ.setLitFor lit bumps).toPropFun :=
+              inf_le_inf (fun τ a => a) hτ₂
+          have : cnfAsListToPropFun Ls ⊓ cnfAsListToPropFun Ls = cnfAsListToPropFun Ls := by simp
+          rw [← inf_assoc, this] at h
+          apply le_trans h ih₁
+        · have := extendsFor_setLitFor_of_none hτ_lit bumps
+          exact extendsFor_trans this ih₂
+      | ⟨τ'', .contra⟩ =>
+        simp
+        replace ih := ih (τ := τ')
+        subst hτ'
+        simp [h_loop] at ih
+        rcases ih with ⟨ih₁, ih₂⟩
+        constructor
+        · have := toPropFun_setLitFor_of_none hτ_lit bumps
+          simp [this] at ih₁ hτ₂
+          clear this h_hint h_loop
+          have := litValue?_none_iff.mp hτ_lit
+          apply le_bot_iff.mp
+          simp [← ih₁, hτ₂]
+        · have := extendsFor_setLitFor_of_none hτ_lit bumps
+          exact extendsFor_trans this ih₂
+    | ⟨τ', .contra⟩ =>
+      simp
+      have h_spec := applyUPHint_spec (τ := τ) h_models hint bumps
+      simp [h_hint] at h_spec
+      rcases h_spec with ⟨hint, h_hint_mem, C, hC, rfl, hC_inf⟩
+      have := cnfPropFun_le_of_mem hC
+      simp [hC_inf] at this
+      simp [this]
+      apply le_bot_iff.mp
+      rw [← hC_inf]
+      exact inf_le_inf_right τ'.toPropFun this
+
+/-! # reduce -/
+
+theorem reduce_loop_eq_reduceM_aux (F : RangeArray ILit) (σ : PS) (hint : Nat)
+  (h_hint : hint < F.size)
+  {Ls : List (Option (List ILit))} {L : List ILit} (h_models : models F Ls L)
+  {C : List ILit} (hC : Ls.get ⟨hint, h_models.h_size₁ ▸ h_hint⟩ = some C)
+  (b : Bool)
+    {i j : Nat}
+    : j = F.rsize hint h_hint - i →
+        RangeArray.reduce.loop F hint σ.mappings σ.gens σ.generation σ.sizes_eq.symm (F.index hint h_hint + i) b =
+        PS.reduce.loop σ { toList := C } i b := by
+  intro hj
+  induction j generalizing i b with
+  | zero =>
+    have h_le := Nat.le_of_sub_eq_zero hj.symm
+    unfold RangeArray.reduce.loop
+    unfold PS.reduce.loop
+    have h_rsize := h_le
+    have h_rsize' := h_models.h_sizes (h_models.h_size₁ ▸ h_hint) hC
+    simp [rsize, Nat.add_comm i] at h_rsize
+    simp [not_lt_of_ge h_rsize, ← h_rsize']
+    intro h_con
+    omega
+  | succ j ih =>
+    have hi : i < F.rsize hint h_hint := by omega
+    have hi' := hi
+    have hj' : j = F.rsize hint h_hint - (i + 1) := by omega
+    simp [rsize] at hi'
+    have : F.index hint h_hint + i < F.index! (hint + 1) := by omega
+    have h_rsize' := h_models.h_sizes (h_models.h_size₁ ▸ h_hint) hC
+    have hiC := h_rsize' ▸ hi
+    unfold RangeArray.reduce.loop
+    unfold PS.reduce.loop
+    simp [← h_rsize', hi, this]
+    have h_hint' := h_models.h_size₁ ▸ h_hint
+    have h_Fget := h_models.h_agree h_hint' hC hiC
+    simp [oget] at h_Fget
+    simp [h_Fget]
+    split_ifs
+
+    · stop
+      rename_i hC_index h_gen_index h_pol
+      split
+      · simp [seval]
+        rename_i h_map
+        unfold PS.litValue PS.litValue_Nat PS.varValue_Nat
+        simp [h_pol, hC_index, LitVar.polarity, h_gen_index]
+        simp [ILit.polarity] at h_pol
+        split at h_pol
+        rename_i lit h_lit h_lit_eq
+        simp at h_pol
+        simp [h_lit_eq] at h_map
+        simp [h_lit_eq, h_pol, h_map]
+      · simp [seval]
+        rename_i h_map
+        unfold PS.litValue PS.litValue_Nat PS.varValue_Nat
+        simp [h_pol, hC_index, LitVar.polarity, h_gen_index]
+        simp [ILit.polarity] at h_pol
+        split at h_pol
+        rename_i lit h_lit h_lit_eq
+        simp at h_pol
+        simp [h_lit_eq] at h_map
+        simp [h_lit_eq, h_pol, h_map]
+        rw [Nat.add_assoc]
+        exact ih true hj'
+      · stop
+        rename_i h_map₀ h_map₁
+        simp [ILit.polarity] at h_pol
+        split at h_pol
+        rename_i lit h_lit h_lit_eq
+        simp at h_pol
+        simp [h_lit_eq, ILit.index] at h_map₀ h_map₁
+        simp [ILitToMappedNat, LitVar.polarity, h_lit_eq, h_pol, ILit.index, seval]
+        unfold PS.litValue PS.litValue_Nat PS.varValue_Nat
+        simp [ILitToMappedNat, LitVar.polarity, h_lit_eq, h_pol, ILit.index, seval, LitVar.toVar]
+        simp [h_lit_eq, ILit.index] at hC_index h_gen_index
+        simp [PSV.fromMappedNat, IVar.index, hC_index, h_gen_index]
+        match h_map_val : σ.mappings[lit.natAbs - 1]'(σ.sizes_eq ▸ hC_index) with
+        | 0 => contradiction
+        | 1 => contradiction
+        | m + 2 =>
+          simp
+          split
+          · split
+            · rename_i h
+              split at h <;> try contradiction
+              · clear h
+                rename_i h; split at h <;> contradiction
+              · split at h <;> contradiction
+            · exact ih b hj'
+            · rename_i h
+              split at h <;> try contradiction
+              · clear h
+                rename_i h
+                split at h <;> contradiction
+              · split at h <;> try contradiction
+                clear h
+                rename_i h _
+                split at h
+                · injection h
+                  rename_i h; subst h
+                  rename_i h
+                  simp [LitVar.mkPos] at h
+                  rename_i h_m2 _ _ hm
+                  simp [Int.natAbs] at h_m2
+                  split at h_m2
+                  · rename_i n
+                    simp [Int.ofNat] at h
+                    have : n = (m + 2) / 2 := by omega
+                    simp at this
+                    have : (⟨↑n, by omega⟩ : ILit) = ⟨↑m / 2 + 1, by omega⟩ := by
+                      simp; omega
+                    exact absurd this h
+                  · omega
+                · injection h
+                  rename_i h; subst h
+                  omega
+          · split
+            · rename_i h
+              split at h
+              · rename_i hm
+                split at hm <;> contradiction
+              · contradiction
+              · split at h <;> simp at h <;> contradiction
+            · rename_i h
+              split at h <;> try contradiction
+              split at h <;> simp at h <;> try contradiction
+              clear h
+              rename_i h; subst h
+              rename_i h
+              split at h
+              · injection h; rename_i h; injection h; rename_i h; subst h; rename_i h
+                simp [Int.natAbs] at h
+                omega
+              · injection h; rename_i h; injection h; rename_i h; subst h; rename_i h
+                simp [Int.ofNat] at h_pol
+                omega
+              done
+            · exact ih true hj'
+    · split
+      · stop
+        rename_i hC_index h_gen_index h_pol n h_map₀
+        simp [ILit.polarity] at h_pol
+        split at h_pol
+        rename_i lit h_lit h_lit_eq
+        simp at h_pol
+        simp [h_lit_eq, ILit.index] at h_map₀
+        simp [ILitToMappedNat, LitVar.polarity, h_lit_eq, h_pol, ILit.index, seval]
+        unfold PS.litValue PS.litValue_Nat PS.varValue_Nat
+        simp [ILitToMappedNat, LitVar.polarity, h_lit_eq, h_pol, ILit.index, seval, LitVar.toVar]
+        simp [h_lit_eq, ILit.index] at hC_index h_gen_index
+        simp [PSV.fromMappedNat, IVar.index, hC_index, h_gen_index, not_lt_of_ge h_pol, negateMappedNat, h_map₀]
+        exact ih true hj'
+      · stop
+        rename_i hC_index h_gen_index h_pol n h_map₁
+        simp [ILit.polarity] at h_pol
+        split at h_pol
+        rename_i lit h_lit h_lit_eq
+        simp at h_pol
+        simp [h_lit_eq, ILit.index] at h_map₁
+        simp [ILitToMappedNat, LitVar.polarity, h_lit_eq, h_pol, ILit.index, seval]
+        unfold PS.litValue PS.litValue_Nat PS.varValue_Nat
+        simp [ILitToMappedNat, LitVar.polarity, h_lit_eq, h_pol, ILit.index, seval, LitVar.toVar]
+        simp [h_lit_eq, ILit.index] at hC_index h_gen_index
+        simp [PSV.fromMappedNat, IVar.index, hC_index, h_gen_index, not_lt_of_ge h_pol, negateMappedNat, h_map₁]
+        done
+      · rename_i hC_index h_gen_index h_pol _ h_map₀ h_map₁
+        simp [ILit.polarity] at h_pol
+        split at h_pol
+        rename_i lit h_lit h_lit_eq
+        simp at h_pol
+        simp [h_lit_eq, ILit.index] at h_map₀ h_map₁
+        simp [ILitToMappedNat, LitVar.polarity, h_lit_eq, h_pol, ILit.index, seval]
+        unfold PS.litValue PS.litValue_Nat PS.varValue_Nat
+        simp [ILitToMappedNat, LitVar.polarity, h_lit_eq, h_pol, ILit.index, seval, LitVar.toVar]
+        simp [h_lit_eq, ILit.index] at hC_index h_gen_index
+        simp [PSV.fromMappedNat, IVar.index, hC_index, h_gen_index, not_lt_of_ge h_pol, negateMappedNat]
+        match h_map_val : σ.mappings[lit.natAbs - 1]'(σ.sizes_eq ▸ hC_index) with
+        | 0 => contradiction
+        | 1 => contradiction
+        | m + 2 =>
+          by_cases h_natAbs : lit.natAbs * 2 + 1 = m + 2
+          <;> simp only [h_natAbs]
+          · simp
+            done
+          · simp
+            split
+            · rename_i h
+              split at h
+              done
+            · rename_i h
+              split at h <;> try contradiction
+              simp at h; subst h
+              rename_i h
+              split at h <;> try contradiction
+              split at h
+              · injection h
+                rename_i h
+                simp [LitVar.mkPos] at h
+                injection h
+                rename_i h; subst h
+                omega
+              · simp [LitVar.mkNeg] at h
+                injection h
+                rename_i h; subst h
+                rename_i n hn2 hn
+                have : -(1 : Int) + -(↑n / 2) = -(1 + n / 2) := by omega
+                split at hn2
+                · simp [Int.natAbs] at h_natAbs
+                  have : m + 1 = n := by omega
+                  subst this
+                  clear hn2
+                  split at h_natAbs
+                  ·
+                    done
+                  · rename_i h
+
+
+                    done
+                  done
+                · omega
+                  done
+                done
+              done
+            done
+          done
+        done
+      done
+    done
+  done
+
+#exit
+
+-- The SR rule
+theorem eqsat_of_SR {F C : PropFun ν} :
+    (∃ σ, F ⊓ Cᶜ ≤ subst (F ⊓ C) σ) → PropFun.EquiSat F (F ⊓ C) := by
+  rintro ⟨σ, hSR⟩
+  constructor
+  · rintro ⟨τ, hτF⟩
+    by_cases hτC : τ ⊨ C
+    · use τ
+      rw [satisfies_conj]
+      exact ⟨hτF, hτC⟩
+    · replace hSR := entails_ext.mp hSR τ
+      simp [satisfies_conj, and_imp, -satisfies_substL] at hSR
+      replace hSR := hSR hτF hτC
+      use PropAssignment.subst σ τ
+      rw [satisfies_conj]
+      exact hSR
+  · rintro ⟨τ, hτ⟩
+    rw [satisfies_conj] at hτ
+    exact ⟨τ, hτ.1⟩
+
+theorem eqsat_of_SR' {F C : PropFun ν} :
+    (∃ σ, F ⊓ Cᶜ ≤ substL (F ⊓ C) σ) → EquiSat F (F ⊓ C) := by
+  rintro ⟨σ, hSR⟩
+  stop
+  constructor
+  · rintro ⟨τ, hτF⟩
+    by_cases hτC : τ ⊨ C
+    · use τ
+      rw [satisfies_conj]
+      exact ⟨hτF, hτC⟩
+    · replace hSR := entails_ext.mp hSR τ
+      simp [satisfies_conj, and_imp, -satisfies_substL] at hSR
+      replace hSR := hSR hτF hτC
+      use PropAssignment.substL (liftSubstL σ) τ
+      rw [satisfies_conj]
+      simp [← subst_liftSubst_eq_substL] at hSR
+      exact hSR
+  · rintro ⟨τ, hτ⟩
+    rw [satisfies_conj] at hτ
+    exact ⟨τ, hτ.1⟩
+
+theorem checkLine_spec {F : RangeArray ILit}
+    {Ls : List (Option (List ILit))} {L : List ILit} (h_models : models F Ls L)
+    (τ : PPA) (σ : PS) (line : Trestle.Parsing.SRAdditionLine)
+  : match checkLine ⟨F, τ, σ⟩ line with
+    | .error false => True
+    | .error true => (cnfAsListToPropFun Ls) = ⊥
+    | .ok ⟨F', τ', σ'⟩ =>
+      F' = F.commit
+      ∧ PropFun.EquiSat (cnfAsListToPropFun Ls) (cnfAsListToPropFun Ls ⊓ clauseAsListToPropFun L)
+  := by
+  -- structure SRAdditionLine where
+  -- witnessLits : Array ILit     -- Maps literals to true/false
+  -- witnessMaps : Array ILit     -- Maps variables to literals
+  -- upHints : Array Nat          -- Already 0-indexed clause IDs into the accumulated formula
+  -- ratHintIndexes : Array Nat   -- Already 0-indexed
+  -- ratHints : Array (Array Nat) -- Already 0-indexed
+  -- ratSizesEq : ratHintIndexes.size = ratHints.size
+  -- witnessMapsMod : witnessMaps.size % 2 = 0
+  --have ⟨witnessLists, witnessMaps, c, d, e, f, g⟩ := line
+  unfold checkLine
+  simp [assumeNegatedCandidateFor_eq_assumeNegatedClauseFor _ _ h_models]
+  match hC : τ.reset.assumeNegatedClauseFor { toList := L } (line.ratHints.size + 1) with
+  | .error τ' => simp
+  | .ok τ' =>
+    simp
+    have := assumeNegatedClauseFor_spec τ.reset L (line.ratHints.size + 1)
+    simp [hC] at this
+    rcases this with ⟨hτ', hτ_extends⟩
+    match h_hints : F.applyUPHints (line.ratHints.size + 1) τ' line.upHints with
+    | ⟨τ'', .err⟩ => simp [h_hints]
+    | ⟨τ'', .unit⟩ =>
+      simp
+      by_cases h_dsize : F.dsize < F.data.size
+      <;> simp [h_dsize]
+      -- Check that we have a nontrivial witness
+      have h_usize : 0 < F.usize := by
+        simp [usize]; exact h_dsize
+      by_cases h_pivot : line.witnessLits[0]?.getD (F.uget 0 h_usize) = F.uget 0 h_usize
+      <;> simp [h_pivot]
+      split <;> try simp
+      rename_i h_loop
+      split at h_loop
+      <;> try (injection h_loop; contradiction)
+      · simp at h_loop
+      rename_i F' τ' σ' h_loop
+      split at h_loop
+      <;> simp at h_loop
+      -- Now check all the RAT/SR hints
+      rcases h_loop with ⟨rfl, rfl, rfl⟩
+      rename_i τ''' h_loop
+      simp
+      apply eqsat_of_SR'
+      use (assumeWitness σ (F.uget 0 h_usize) line.witnessLits line.witnessMaps).toSubst
+
+      done
+    | ⟨τ'', .contra⟩ =>
+      simp
+      have := applyUPHints_spec (τ := τ') h_models (line.ratHints.size + 1) line.upHints.toList
+      simp [h_hints] at this
+      rcases this with ⟨h_hints₁, h_hints₂⟩
+      by_cases h_usize : F.usize = 0
+      -- Trivial branch: If the candidate is empty, we should have found contradiction by now
+      · simp [h_usize]
+        simp [h_models.h_size₂] at h_usize
+        subst h_usize
+        simp at hτ'
+        simp [hτ'] at h_hints₁
+        exact h_hints₁
+      -- UP Contradiction branch: we return immediately; check for equisat
+      · simp [h_usize]
+        apply equisat_of_entails
+        simp [hτ'] at h_hints₁
+        exact le_iff_inf_compl_eq_bot.mpr h_hints₁
+      done
+    done
+  done
+
+end Trestle.SR
